src/tls/Crypto.AE.fsti
@@ -1,0 +1,47 @@
+module Crypto.AE
+include Crypto.AEAD
+
+module U8 = FStar.UInt8
+module Seq = FStar.Seq
+module SC = Spec.AEAD
+module B = LowStar.Buffer
+module U32 = FStar.UInt32
+module HS = FStar.HyperStack
+module HST = FStar.HyperStack.ST
+module EE = EverCrypt.Error
+module G = FStar.Ghost
+module F = Flags
+module Cast = Crypto.Util.IntCast
+
+val encrypt
+  (#a: SC.supported_alg)
+  (#phi: plain_pred)
+  (s: state a phi) // key
+  (plain: plain_p a)
+  (plain_len: U32.t {U32.v plain_len == B.length plain})
+  (cipher: cipher_p a) // cipher == iv ++ cipher ++ tag (see EverCrypt.AEAD.encrypt_st)
+: HST.Stack EE.error_code
+  (requires (fun h ->
+    invariant h s /\
+    B.live h plain /\
+    B.live h cipher /\
+    phi (B.as_seq h plain) /\
+    B.loc_disjoint (footprint s) (B.loc_buffer plain) /\
+    B.loc_disjoint (footprint s) (B.loc_buffer cipher) /\
+    B.disjoint plain cipher /\
+    B.length cipher == B.length plain + iv_length + SC.tag_length a
+  ))
+  (ensures (fun h res h' -> 
+    match res with
+    | EE.InvalidKey ->
+      B.modifies (B.loc_buffer cipher) h h' // TODO: should be False, need to fix EverCrypt
+    | EE.Success ->
+      let iv = B.gsub cipher 0ul iv_len in
+      let cipher' = B.gsub cipher iv_len (B.len cipher `U32.sub` iv_len) in
+      B.modifies (B.loc_union (footprint s) (B.loc_buffer cipher)) h h' /\
+      invariant h' s /\
+      (F.ideal_AEAD == false ==> SC.encrypt (state_kv s) (Cast.to_seq_sec8 (B.as_seq h' iv)) Seq.empty (Cast.to_seq_sec8 (B.as_seq h plain)) `Seq.equal` Cast.to_seq_sec8 (B.as_seq h' cipher'))
+    | _ -> False
+  ))
+
+// decrypt is unchanged from Crypto.AEAD.decrypt
